theories/simplang/primitive_laws.v
@@ -19,19 +19,17 @@ Class sheapG (Σ: gFunctors) := SHeapG {
    It states additional components of the state interpretation, i.e.,
    invariants on the relation of source and target programs and states.
  *)
-Class sheapRel (Σ : gFunctors) := SHeapRel {
-  sheap_stateRel : state → state → iProp Σ;
-  sheap_progRel : prog → prog → iProp Σ;
+Class sheapInv (Σ : gFunctors) := SHeapRel {
+  sheap_inv : iProp Σ;
 }.
 
-Global Instance sheapG_SimulLang `{!sheapG Σ} `{!sheapRel Σ} : SimulLang (iPropI Σ) simp_lang := {
+Global Instance sheapG_SimulLang `{!sheapG Σ} `{!sheapInv Σ} : SimulLang (iPropI Σ) simp_lang := {
   state_interp P_t σ_t P_s σ_s :=
     (gen_prog_interp (hG := gen_prog_inG_target) P_t ∗
      gen_prog_interp (hG := gen_prog_inG_source) P_s ∗
      gen_heap_interp (hG := gen_heap_inG_target) σ_t.(heap) ∗
      gen_heap_interp (hG := gen_heap_inG_source) σ_s.(heap) ∗
-     sheap_stateRel σ_t σ_s ∗
-     sheap_progRel P_t P_s
+     sheap_inv
     )%I;
 }.
 
@@ -63,7 +61,7 @@ Notation "f '@s' Ks" := (hasfun (hG:=gen_prog_inG_source) f Ks)
   (at level 20, format "f  @s  Ks") : bi_scope.
 
 Section lifting.
-Context `{!sheapG Σ} `{!sheapRel Σ}.
+Context `{!sheapG Σ} `{!sheapInv Σ}.
 Implicit Types P Q : iProp Σ.
 Implicit Types Φ : val → val → iProp Σ.
 Implicit Types σ σ_s σ_t : state.
@@ -162,32 +160,29 @@ Qed.
 
 Lemma target_red_allocN_seq n v Ψ :
   (0 < n)%Z →
-  (∀ σ_t σ_s l, sheap_stateRel σ_t σ_s -∗ sheap_stateRel (state_init_heap l n v σ_t) σ_s) -∗
   (∀ l, ([∗ list] i ∈ seq 0 (Z.to_nat n), (l +ₗ (i : nat)) ↦t v) -∗
     target_red (of_val #l) Ψ) -∗
   target_red (AllocN (Val $ LitV $ LitInt $ n) (Val v)) Ψ.
 Proof.
-  iIntros (Hn) "Hrel Hloc". iApply target_red_lift_head_step.
-  iIntros (P_s σ_s P_t σ_t) "(HP_t & HP_s & Hσ_t & Hσ_s & Hstate & Hprog)". iModIntro.
+  iIntros (Hn) "Hloc". iApply target_red_lift_head_step.
+  iIntros (P_s σ_s P_t σ_t) "(HP_t & HP_s & Hσ_t & Hσ_s & Hinv)". iModIntro.
   iSplitR. { iPureIntro. eauto with lia head_step. }
   iIntros (e_t' σ_t') "%"; inv_head_step.
   iMod (gen_heap_alloc_big _ (heap_array l (replicate (Z.to_nat n) v)) with "Hσ_t")
     as "(Hσ_t & Hl & Hm)".
   { apply heap_array_map_disjoint. rewrite replicate_length Z2Nat.id; auto with lia. }
   iPoseProof (heap_array_to_seq_mapsto with "Hl") as "Hmap".
-  iModIntro. iFrame. iSplitL "Hrel Hstate"; first by iApply "Hrel".
-  by iApply "Hloc".
+  iModIntro. iFrame. by iApply "Hloc".
 Qed.
 
 Lemma source_red_allocN_seq n v Ψ :
   (0 < n)%Z →
-  (∀ σ_t σ_s l, sheap_stateRel σ_t σ_s -∗ sheap_stateRel σ_t (state_init_heap l n v σ_s)) -∗
   (∀ l, ([∗ list] i ∈ seq 0 (Z.to_nat n), (l +ₗ (i : nat)) ↦s v) -∗
     source_red (of_val #l) Ψ) -∗
   source_red (AllocN (Val $ LitV $ LitInt $ n) (Val v)) Ψ.
 Proof.
-  iIntros (Hn) "Hrel Hloc". iApply source_red_lift_head_step.
-  iIntros (P_s σ_s P_t σ_t) "[(HP_t & HP_s & Hσ_t & Hσ_s & Hstate & Hprog) _]".
+  iIntros (Hn) "Hloc". iApply source_red_lift_head_step.
+  iIntros (P_s σ_s P_t σ_t) "[(HP_t & HP_s & Hσ_t & Hσ_s & Hinv) _]".
   assert (head_reducible P_s (AllocN #n v) σ_s) as (e_s' & σ_s' & Hred).
   { eauto with lia head_step. }
   inv_head_step.
@@ -196,55 +191,51 @@ Proof.
   { apply heap_array_map_disjoint. rewrite replicate_length Z2Nat.id; auto with lia. }
   iModIntro. iExists #l, (state_init_heap l n v σ_s).
   iSplitR. { eauto with lia head_step. }
-  iFrame. iModIntro. iSplitL "Hstate Hrel"; first by iApply "Hrel".
+  iFrame. iModIntro.
   iApply "Hloc". iApply (heap_array_to_seq_mapsto with "Hl").
 Qed.
 
 Lemma target_red_alloc v Ψ :
-  (∀ σ_t σ_s l, sheap_stateRel σ_t σ_s -∗ sheap_stateRel (state_init_heap l 1 v σ_t) σ_s) -∗
   (∀ l, l ↦t v -∗ target_red (of_val #l) Ψ) -∗
   target_red (Alloc (Val v)) Ψ.
 Proof.
-  iIntros "Hrel Ht". iApply (target_red_allocN_seq with "Hrel"); first lia.
+  iIntros "Ht". iApply (target_red_allocN_seq); first lia.
   iIntros (l) "[Hl _]". iApply "Ht". by rewrite loc_add_0.
 Qed.
 
 Lemma source_red_alloc v Ψ :
-  (∀ σ_t σ_s l, sheap_stateRel σ_t σ_s -∗ sheap_stateRel σ_t (state_init_heap l 1 v σ_s)) -∗
   (∀ l, l ↦s v -∗ source_red (of_val #l) Ψ) -∗
   source_red (Alloc (Val v)) Ψ.
 Proof.
-  iIntros "Hrel Ht". iApply (source_red_allocN_seq with "Hrel"); first lia.
+  iIntros "Ht". iApply (source_red_allocN_seq); first lia.
   iIntros (l) "[Hl _]". iApply "Ht". by rewrite loc_add_0.
 Qed.
 
 Lemma target_red_free v l Ψ :
-  (∀ σ_t σ_s, sheap_stateRel σ_t σ_s -∗ sheap_stateRel (state_upd_heap <[l:=None]> σ_t) σ_s) -∗
   l ↦t v -∗ target_red (of_val #()) Ψ -∗
   target_red (Free (Val $ LitV (LitLoc l))) Ψ.
 Proof.
-  iIntros "Hrel Hl Hsim". iApply target_red_lift_head_step.
-  iIntros (????) "(HP_t & HP_s & Hσ_t & Hσ_s & Hstate & Hprog)".
+  iIntros "Hl Hsim". iApply target_red_lift_head_step.
+  iIntros (????) "(HP_t & HP_s & Hσ_t & Hσ_s & Hinv)".
   iDestruct (gen_heap_valid with "Hσ_t Hl") as %?.
   iModIntro. iSplitR; first by eauto with head_step.
   iIntros (e_t' σ_t') "%"; inv_head_step.
   iMod (gen_heap_update with "Hσ_t Hl") as "[$ Hl]".
-  iModIntro. iFrame. by iApply "Hrel".
+  iModIntro. iFrame.
 Qed.
 
 Lemma source_red_free v l Ψ :
-  (∀ σ_t σ_s, sheap_stateRel σ_t σ_s -∗ sheap_stateRel σ_t (state_upd_heap <[l:=None]> σ_s)) -∗
   l ↦s v -∗ source_red (of_val #()) Ψ -∗
   source_red (Free (Val $ LitV (LitLoc l))) Ψ.
 Proof.
-  iIntros "Hrel Hl Hsim". iApply source_red_lift_head_step.
-  iIntros (????) "[(HP_t & HP_s & Hσ_t & Hσ_s & Hstate & Hprog) _]".
+  iIntros "Hl Hsim". iApply source_red_lift_head_step.
+  iIntros (????) "[(HP_t & HP_s & Hσ_t & Hσ_s & Hinv) _]".
   iModIntro. iDestruct (gen_heap_valid with "Hσ_s Hl") as %?.
   assert (head_reducible P_s (Free #l) σ_s) as (e_s' & σ_s' & Hred).
   { eauto with head_step. }
   iExists e_s', σ_s'. iSplitR; first done.
   inv_head_step. iMod (gen_heap_update with "Hσ_s Hl") as "[$ Hl]".
-  iModIntro. iFrame. by iApply "Hrel".
+  iModIntro. iFrame.
 Qed.
 
 Lemma target_red_load l dq v Ψ :
@@ -253,7 +244,7 @@ Lemma target_red_load l dq v Ψ :
   target_red (Load (Val $ LitV $ LitLoc l)) Ψ.
 Proof.
   iIntros "Hl Ht". iApply target_red_lift_head_step.
-  iIntros (????) "(HP_t & HP_s & Hσ_t & Hσ_s & Hstate & Hprog)".
+  iIntros (????) "(HP_t & HP_s & Hσ_t & Hσ_s & Hinv)".
   iDestruct (gen_heap_valid with "Hσ_t Hl") as %?. iModIntro.
   iSplit; first by eauto with head_step.
   iIntros (?? Hstep); inv_head_step.
@@ -266,7 +257,7 @@ Lemma source_red_load l dq v Ψ :
   source_red (Load (Val $ LitV $ LitLoc l)) Ψ.
 Proof.
   iIntros "Hl Ht". iApply source_red_lift_head_step.
-  iIntros (????) "[(HP_t & HP_s & Hσ_t & Hσ_s & Hstate & Hprog) _]".
+  iIntros (????) "[(HP_t & HP_s & Hσ_t & Hσ_s & Hinv) _]".
   iDestruct (gen_heap_valid with "Hσ_s Hl") as %?.
   assert (head_reducible P_s (Load #l) σ_s) as (e_s' & σ_s' & Hred).
   { eauto with head_step. }
@@ -275,36 +266,32 @@ Proof.
 Qed.
 
 Lemma target_red_store l v v' Ψ :
-  (∀ σ_t σ_s, sheap_stateRel σ_t σ_s -∗ sheap_stateRel (state_upd_heap <[l:=Some v]> σ_t) σ_s) -∗
   l ↦t v' -∗
   (l ↦t v -∗ target_red (of_val #()) Ψ) -∗
   target_red (Store (Val $ LitV (LitLoc l)) (Val v)) Ψ.
 Proof.
-  iIntros "Hrel Hl Hsim". iApply target_red_lift_head_step.
-  iIntros (????) "(HP_t & HP_s & Hσ_t & Hσ_s & Hstate & Hprog) !>".
+  iIntros "Hl Hsim". iApply target_red_lift_head_step.
+  iIntros (????) "(HP_t & HP_s & Hσ_t & Hσ_s & Hinv) !>".
   iDestruct (gen_heap_valid with "Hσ_t Hl") as %?.
   iSplitR; first by eauto with head_step.
   iIntros (e_t' σ_t') "%"; inv_head_step.
   iMod (gen_heap_update with "Hσ_t Hl") as "[$ Hl]".
-  iModIntro. iFrame. iSplitL "Hrel Hstate"; first by iApply "Hrel".
-  by iApply "Hsim".
+  iModIntro. iFrame. by iApply "Hsim".
 Qed.
 
 Lemma source_red_store l v v' Ψ :
-  (∀ σ_t σ_s, sheap_stateRel σ_t σ_s -∗ sheap_stateRel σ_t (state_upd_heap <[l:=Some v]> σ_s)) -∗
   l ↦s v' -∗
   (l ↦s v -∗ source_red (of_val #()) Ψ) -∗
   source_red (Store (Val $ LitV (LitLoc l)) (Val v)) Ψ.
 Proof.
-  iIntros "Hrel Hl Hsim". iApply source_red_lift_head_step.
-  iIntros (????) "[(HP_t & HP_s & Hσ_t & Hσ_s & Hstate & Hprog) _] !>".
+  iIntros "Hl Hsim". iApply source_red_lift_head_step.
+  iIntros (????) "[(HP_t & HP_s & Hσ_t & Hσ_s & Hinv) _] !>".
   iDestruct (gen_heap_valid with "Hσ_s Hl") as %?.
   assert (head_reducible P_s (Store (Val $ LitV (LitLoc l)) (Val v)) σ_s) as (e_s' & σ_s' & Hred).
   { eauto with head_step. }
   iExists e_s', σ_s'. iSplitR; first done. inv_head_step.
   iMod (gen_heap_update with "Hσ_s Hl") as "[$ Hl]".
-  iModIntro. iFrame. iSplitL "Hstate Hrel"; first by iApply "Hrel".
-  by iApply "Hsim".
+  iModIntro. iFrame. by iApply "Hsim".
 Qed.
 
 (** operational lemmas for calls *)
@@ -314,7 +301,7 @@ Lemma target_red_call f K_t v Ψ :
   target_red (Call (Val $ LitV $ LitFn f) (Val v)) Ψ.
 Proof.
   iIntros "Hf Hred". iApply target_red_lift_head_step.
-  iIntros (????) "(HP_t & HP_s & Hσ_t & Hσ_s & ? & ?) !>".
+  iIntros (????) "(HP_t & HP_s & Hσ_t & Hσ_s & ?) !>".
   iDestruct (gen_prog_valid with "HP_t Hf") as %?.
   iSplitR; first by eauto with head_step.
   iIntros (e_t' σ_t') "%"; inv_head_step.
@@ -327,7 +314,7 @@ Lemma source_red_call f K_s v Ψ :
   source_red (Call (Val $ LitV $ LitFn f) (Val v)) Ψ.
 Proof.
   iIntros "Hf Hred". iApply source_red_lift_head_step.
-  iIntros (????) "[(HP_t & HP_s & Hσ_t & Hσ_s & ? & ?) _] !>".
+  iIntros (????) "[(HP_t & HP_s & Hσ_t & Hσ_s & ?) _] !>".
   iDestruct (gen_prog_valid with "HP_s Hf") as %?.
   assert (head_reducible P_s (Call (Val $ LitV $ LitFn f) (Val v)) σ_s) as (e_s' & σ_s' & Hred).
   { eauto with head_step. }
